Refactory directory structure

Phi_Semantics/PhiSem_Variable.thy
@@ -283,6 +283,162 @@ lemma op_free_var:
 
 
 
+section \<open>IDE-CP Operations\<close>
+
+subsection \<open>Syntax\<close>
+
+lemma [\<phi>reason 2000 for
+  \<open>Synthesis_Parse (?var::varname) (?Y::?'ret \<Rightarrow> assn)\<close>
+]:
+  \<open>Synthesis_Parse var (\<lambda>_. x \<Ztypecolon> Var var T :: assn)\<close>
+  unfolding Synthesis_Parse_def ..
+
+subsection \<open>Reasoning Process\<close>
+
+subsubsection \<open>Infer Semantic Type of Variable\<close>
+
+consts infer_var_type :: \<open>unit action\<close>
+
+lemma [\<phi>reason 1000]:
+  \<open> varname.type var \<equiv> TY'
+\<Longrightarrow> pred_option ((=) TY) TY' \<^bold><\<^bold>a\<^bold>c\<^bold>t\<^bold>i\<^bold>o\<^bold>n\<^bold>> infer_var_type
+\<Longrightarrow> pred_option ((=) TY) (varname.type var) \<^bold><\<^bold>a\<^bold>c\<^bold>t\<^bold>i\<^bold>o\<^bold>n\<^bold>> infer_var_type\<close>
+  \<comment> \<open>TY is the output. The rule invokes evaluation of the \<open>varname.type var\<close>.\<close>
+  by simp
+
+lemma [\<phi>reason 1000]:
+  \<open>pred_option ((=) TY) None \<^bold><\<^bold>a\<^bold>c\<^bold>t\<^bold>i\<^bold>o\<^bold>n\<^bold>> infer_var_type\<close>
+  \<comment> \<open>the output TY can be anything freely\<close>
+  by simp
+
+lemma [\<phi>reason 1000 for \<open>pred_option ((=) ?TY') (Some ?TY) \<^bold><\<^bold>a\<^bold>c\<^bold>t\<^bold>i\<^bold>o\<^bold>n\<^bold>> infer_var_type\<close>]:
+  \<open>pred_option ((=) TY) (Some TY) \<^bold><\<^bold>a\<^bold>c\<^bold>t\<^bold>i\<^bold>o\<^bold>n\<^bold>> infer_var_type\<close>
+  \<comment> \<open>the output TY equals to that TY in \<open>Some TY\<close> exactly.\<close>
+  by simp
+
+lemma
+  \<open>pred_option (\<lambda>TY'. TY = TY') None\<close>
+  \<open>pred_option (\<lambda>TY'. TY = TY') (Some TY)\<close>
+  by simp+
+
+
+subsection \<open>Rules of Variable Operations\<close>
+
+subsubsection \<open>Get\<close>
+
+proc (nodef) op_get_var:
+  assumes [unfolded \<phi>SemType_def subset_iff, useful]: \<open>\<phi>SemType (x \<Ztypecolon> T) TY\<close>
+  argument \<open>x \<Ztypecolon> \<^bold>v\<^bold>a\<^bold>r[var] T\<close>
+  return   \<open>x \<Ztypecolon> \<^bold>v\<^bold>a\<^bold>r[var] T\<heavy_comma> x \<Ztypecolon> \<^bold>v\<^bold>a\<^bold>l T\<close>
+  \<medium_left_bracket> to_Identity op_get_var'' \<medium_right_bracket>. .
+
+lemma [\<phi>reason 1200 for
+    \<open>\<^bold>p\<^bold>r\<^bold>o\<^bold>c ?f \<lbrace> ?R \<longmapsto> \<lambda>ret. ?R'\<heavy_comma> SYNTHESIS ?x <val-of> ?var \<Ztypecolon> ?T ret \<^bold>t\<^bold>h\<^bold>r\<^bold>o\<^bold>w\<^bold>s ?E \<rbrace> \<^bold>@\<^bold>G\<^bold>O\<^bold>A\<^bold>L ?G\<close>
+]:
+  \<open> SUBGOAL G G2
+\<Longrightarrow> \<^bold>v\<^bold>i\<^bold>e\<^bold>w X \<longmapsto> Y\<heavy_comma> \<blangle> x \<Ztypecolon> \<^bold>v\<^bold>a\<^bold>r[var] T \<brangle> \<^bold><\<^bold>a\<^bold>c\<^bold>t\<^bold>i\<^bold>o\<^bold>n\<^bold>> reason_ToSA True G2
+\<Longrightarrow> SOLVE_SUBGOAL G2
+\<Longrightarrow> \<phi>SemType (x \<Ztypecolon> T) TY
+\<Longrightarrow> \<^bold>p\<^bold>r\<^bold>o\<^bold>c op_get_var var TY \<lbrace> X \<longmapsto> Y\<heavy_comma> x \<Ztypecolon> \<^bold>v\<^bold>a\<^bold>r[var] T \<heavy_comma> SYNTHESIS \<^bold>v\<^bold>a\<^bold>l x <val-of> var \<Ztypecolon> T \<rbrace> \<^bold>@\<^bold>G\<^bold>O\<^bold>A\<^bold>L G\<close>
+  unfolding Action_Tag_def
+  \<medium_left_bracket> premises _ and GetVar and _ and [\<phi>reason for \<open>\<phi>SemType (x \<Ztypecolon> T) ?TY\<close>]
+    GetVar op_get_var \<medium_right_bracket>. .
+
+
+
+subsubsection \<open>Set\<close>
+
+proc (nodef) op_set_var:
+  assumes [unfolded Action_Tag_def, useful]:
+      \<open>pred_option (\<lambda>TY'. TY = TY') (varname.type var) \<^bold><\<^bold>a\<^bold>c\<^bold>t\<^bold>i\<^bold>o\<^bold>n\<^bold>> infer_var_type\<close>
+  assumes [unfolded \<phi>SemType_def subset_iff, useful]:
+      \<open>\<phi>SemType (y \<Ztypecolon> U) TY\<close>
+  argument \<open>x \<Ztypecolon> Var var T\<heavy_comma> \<^bold>v\<^bold>a\<^bold>l y \<Ztypecolon> U\<close>
+  return   \<open>y \<Ztypecolon> \<^bold>v\<^bold>a\<^bold>r[var] U\<close>
+  \<medium_left_bracket> to_Identity 
+    $y to_Identity
+    op_set_var'' 
+  \<medium_right_bracket>. .
+
+schematic_goal op_set_var__synthesis [\<phi>reason 1200 for 
+  \<open>\<^bold>p\<^bold>r\<^bold>o\<^bold>c ?f \<lbrace> ?R \<longmapsto> \<lambda>ret. ?R'\<heavy_comma> SYNTHESIS (?y <set-to> ?var) \<Ztypecolon> ?U ret \<^bold>t\<^bold>h\<^bold>r\<^bold>o\<^bold>w\<^bold>s ?E \<rbrace> \<^bold>@\<^bold>G\<^bold>O\<^bold>A\<^bold>L ?G\<close>
+]:
+assumes G: \<open>\<^bold>p\<^bold>r\<^bold>o\<^bold>c g \<lbrace> X \<longmapsto> X1\<heavy_comma> SYNTHESIS \<^bold>v\<^bold>a\<^bold>l y \<Ztypecolon> U \<^bold>t\<^bold>h\<^bold>r\<^bold>o\<^bold>w\<^bold>s E\<rbrace> \<^bold>@\<^bold>G\<^bold>O\<^bold>A\<^bold>L G \<close>
+  and P: \<open>pred_option (\<lambda>TY'. TY = TY') (varname.type var) \<^bold><\<^bold>a\<^bold>c\<^bold>t\<^bold>i\<^bold>o\<^bold>n\<^bold>> infer_var_type\<close>
+  and S[unfolded Action_Tag_def]:
+         \<open>\<^bold>v\<^bold>i\<^bold>e\<^bold>w X1 \<longmapsto> Y\<heavy_comma> x \<Ztypecolon> Var var T \<^bold>w\<^bold>i\<^bold>t\<^bold>h Any \<^bold><\<^bold>a\<^bold>c\<^bold>t\<^bold>i\<^bold>o\<^bold>n\<^bold>> ToSA\<close>
+  and [\<phi>reason for \<open>\<phi>SemType (y \<Ztypecolon> U) ?TY\<close>]:
+         \<open>\<phi>SemType (y \<Ztypecolon> U) TY\<close>
+shows \<open>\<^bold>p\<^bold>r\<^bold>o\<^bold>c ?FF \<lbrace> X \<longmapsto> Y\<heavy_comma> y \<Ztypecolon> \<^bold>v\<^bold>a\<^bold>r[var] U \<heavy_comma> SYNTHESIS \<^bold>v\<^bold>a\<^bold>l (y <set-to> var) \<Ztypecolon> U \<^bold>t\<^bold>h\<^bold>r\<^bold>o\<^bold>w\<^bold>s E \<rbrace> \<^bold>@\<^bold>G\<^bold>O\<^bold>A\<^bold>L G\<close>
+  \<medium_left_bracket> G S op_set_var P op_get_var \<medium_right_bracket>. .
+
+
+subsubsection \<open>Declare New Variables\<close>
+
+proc op_var_scope:
+  assumes BLK: \<open>\<And>var. varname.type var \<equiv> TY
+                  \<Longrightarrow> \<^bold>p\<^bold>r\<^bold>o\<^bold>c F var \<lbrace> X\<heavy_comma> \<^bold>u\<^bold>n\<^bold>i\<^bold>n\<^bold>i\<^bold>t\<^bold>e\<^bold>d \<^bold>v\<^bold>a\<^bold>r[var] \<longmapsto> \<lambda>ret. Y ret\<heavy_comma> () \<Ztypecolon> Var var \<phi>Any
+                      \<^bold>t\<^bold>h\<^bold>r\<^bold>o\<^bold>w\<^bold>s \<lambda>v. E v \<heavy_comma> () \<Ztypecolon> Var var \<phi>Any \<rbrace>\<close>
+  argument \<open>X\<close>
+  return   \<open>Y\<close>
+  throws   E
+  \<medium_left_bracket> op_var_scope'[where TY=TY]
+    try''
+    \<medium_left_bracket> premises [\<phi>reason]
+      BLK to_Identity op_free_var
+    \<medium_right_bracket>.
+    \<medium_left_bracket> to_Identity op_free_var throw \<medium_right_bracket>.
+  \<medium_right_bracket>. .
+
+subsection \<open>Implementing IDE-CP Generic Variable Access\<close>
+
+lemma "__new_var_rule__":
+  \<open> (\<And>var. varname.type var \<equiv> TY
+              \<Longrightarrow> \<^bold>p\<^bold>r\<^bold>o\<^bold>c g var \<lbrace> R\<heavy_comma> \<^bold>u\<^bold>n\<^bold>i\<^bold>n\<^bold>i\<^bold>t\<^bold>e\<^bold>d \<^bold>v\<^bold>a\<^bold>r[var]\<heavy_comma> X \<longmapsto> \<lambda>ret. Z ret \<heavy_comma> () \<Ztypecolon> Var var \<phi>Any
+                             \<^bold>t\<^bold>h\<^bold>r\<^bold>o\<^bold>w\<^bold>s \<lambda>e. E e\<heavy_comma> () \<Ztypecolon> Var var \<phi>Any \<rbrace>)
+\<Longrightarrow> \<^bold>p\<^bold>r\<^bold>o\<^bold>c op_var_scope TYPE('a) TY g \<lbrace> R\<heavy_comma> X \<longmapsto> Z \<^bold>t\<^bold>h\<^bold>r\<^bold>o\<^bold>w\<^bold>s E \<rbrace>\<close>
+  \<medium_left_bracket> premises G
+    op_var_scope[where TY=\<open>TY\<close>] \<medium_left_bracket> premises [\<phi>reason for \<open>varname.type var \<equiv> _\<close>] G \<medium_right_bracket>.
+  \<medium_right_bracket>. .
+
+
+lemma "__set_var_rule__":
+  \<open> \<^bold>p\<^bold>r\<^bold>o\<^bold>c g \<lbrace> R\<heavy_comma> y \<Ztypecolon> \<^bold>v\<^bold>a\<^bold>r[var] U\<heavy_comma> X \<longmapsto> Z \<^bold>t\<^bold>h\<^bold>r\<^bold>o\<^bold>w\<^bold>s E \<rbrace>
+\<Longrightarrow> pred_option (\<lambda>TY'. TY = TY') (varname.type var) \<^bold><\<^bold>a\<^bold>c\<^bold>t\<^bold>i\<^bold>o\<^bold>n\<^bold>> infer_var_type
+\<Longrightarrow> \<phi>SemType (y \<Ztypecolon> U) TY
+\<Longrightarrow> \<^bold>p\<^bold>r\<^bold>o\<^bold>c (op_set_var var TY raw \<ggreater> g) \<lbrace> R\<heavy_comma> (x \<Ztypecolon> Var var T \<heavy_comma> y \<Ztypecolon> \<^bold>v\<^bold>a\<^bold>l[raw] U\<heavy_comma> X) \<longmapsto> Z \<^bold>t\<^bold>h\<^bold>r\<^bold>o\<^bold>w\<^bold>s E \<rbrace>\<close>
+  \<medium_left_bracket> premises G and P and [\<phi>reason for \<open>\<phi>SemType (y \<Ztypecolon> U) ?TY\<close>]
+    op_set_var P G  \<medium_right_bracket>. .
+
+lemma "__set_new_var_rule__":
+  \<open> (\<And>var. varname.type var \<equiv> Some TY
+              \<Longrightarrow> \<^bold>p\<^bold>r\<^bold>o\<^bold>c g var \<lbrace> R\<heavy_comma> y \<Ztypecolon> \<^bold>v\<^bold>a\<^bold>r[var] U\<heavy_comma> X \<longmapsto> \<lambda>ret. Z ret \<heavy_comma> () \<Ztypecolon> Var var \<phi>Any
+                             \<^bold>t\<^bold>h\<^bold>r\<^bold>o\<^bold>w\<^bold>s \<lambda>e. E e\<heavy_comma> () \<Ztypecolon> Var var \<phi>Any \<rbrace>)
+\<Longrightarrow> \<phi>SemType (y \<Ztypecolon> U) TY
+\<Longrightarrow> \<^bold>p\<^bold>r\<^bold>o\<^bold>c op_var_scope TYPE('a) (Some TY) (\<lambda>var. op_set_var var TY raw \<ggreater> g var)
+     \<lbrace> R\<heavy_comma> (y \<Ztypecolon> \<^bold>v\<^bold>a\<^bold>l[raw] U\<heavy_comma> X) \<longmapsto> Z \<^bold>t\<^bold>h\<^bold>r\<^bold>o\<^bold>w\<^bold>s E \<rbrace>\<close>
+  \<medium_left_bracket> premises G and [\<phi>reason]
+    op_var_scope[where TY=\<open>Some TY\<close>] \<medium_left_bracket> premises [\<phi>reason for \<open>varname.type var \<equiv> _\<close>]
+      $y op_set_var G
+    \<medium_right_bracket>.
+  \<medium_right_bracket>. .
+
+lemma "__set_new_var_noty_rule__":
+  \<open> (\<And>var. varname.type var \<equiv> None
+              \<Longrightarrow> \<^bold>p\<^bold>r\<^bold>o\<^bold>c g var \<lbrace> R\<heavy_comma> y \<Ztypecolon> \<^bold>v\<^bold>a\<^bold>r[var] U\<heavy_comma> X \<longmapsto> \<lambda>ret. Z ret \<heavy_comma> () \<Ztypecolon> Var var \<phi>Any
+                             \<^bold>t\<^bold>h\<^bold>r\<^bold>o\<^bold>w\<^bold>s \<lambda>e. E e\<heavy_comma> () \<Ztypecolon> Var var \<phi>Any \<rbrace>)
+\<Longrightarrow> \<phi>SemType (y \<Ztypecolon> U) TY
+\<Longrightarrow> \<^bold>p\<^bold>r\<^bold>o\<^bold>c op_var_scope TYPE('a) None (\<lambda>var. op_set_var var TY raw \<ggreater> g var)
+     \<lbrace> R\<heavy_comma> (y \<Ztypecolon> \<^bold>v\<^bold>a\<^bold>l[raw] U\<heavy_comma> X) \<longmapsto> Z \<^bold>t\<^bold>h\<^bold>r\<^bold>o\<^bold>w\<^bold>s E \<rbrace>\<close>
+  \<medium_left_bracket> premises G and [\<phi>reason for \<open>\<phi>SemType (y \<Ztypecolon> U) _\<close>]
+    op_var_scope[where TY=None] \<medium_left_bracket> premises [\<phi>reason for \<open>varname.type var \<equiv> _\<close>]
+      $y op_set_var G
+    \<medium_right_bracket>.
+  \<medium_right_bracket>. .
+
+ML_file "library/variable.ML"
+
+
 end
 
 
